%\footnotesize
\begin{dmath}
% Equation 1
Z=\sum_{t = 0}^{\infty} \beta^{t} \Big[(log(c_{t}) - \frac{A^{L}\epsilon^{L_{t}}\Big[\sum_{k} n_{k,t}\Big]^{1 + \sigma^{L}}}{1 + \sigma^{L}} \Big]
\end{dmath}
\begin{dmath}
% Equation 2
c_{t} = Y_{t}
\end{dmath}
\begin{dmath}
% Equation 3
Y_{t}=  \sum_{k} w_{k,t} y_{k,t} 
\end{dmath}
\begin{dmath}
% Equation 4
N_{t} = \sum_{k}  n_{k,t}
\end{dmath}
\begin{dmath}
% Equation 5
H_{t} =  \sum_{k}  h_{k,t}
\end{dmath}
\begin{dmath}
% Equation 6
U_{t} = 1-(1-\delta)N_{t-1}
\end{dmath}
\begin{dmath}
% Equation 7
y_{k,t} = \epsilon_{k,t} \, a_{k} n_{k,t}^{\alpha_{k}} \, \prod_{j=1}^{M} x_{k,j,t}^{\gamma_{k,j}}-\sum_{j=1}^{M} x_{j,k,t} -\frac{mch_{t} h_{k,t}^{\psi}}{\psi} 
\end{dmath}
\begin{dmath}
% Equation 8
h_{k,t}=n_{k,t}-(1-\delta)n_{k,t-1}
\end{dmath}
\begin{dmath}
% Equation 9
mch_{t}=\frac{\xi}{\nu}\Big(\frac{H_{t}}{U_{t}}\Big)^{\nu}
\end{dmath}
\begin{dmath}
% Equation 10
\frac{{w_{k,t}}\, {\alpha_{k}}\, \epsilon_{k,t} \, a_{k} \, n_{k,t}^{{\alpha_{k}}-1} \prod_{j=1}^{M} x_{k,j,t}^{\gamma_{k, j}} - mch_{t} \, h_{k,t}^{{\psi}-1}}{Y_{t}}+\frac{(1-{\delta})\, {w_{k,t}}\, {\beta}\, mch_{t+1}\, {h_{k,t+1}^{{\psi}-1}}}{Y_{t+1}}=\,A^{L}\epsilon^{L}_{t}N_{k,t}^{\sigma^{L}}
\end{dmath}
\begin{dmath}
% Equation 11
\epsilon_{k,t}\, {a_{k}}\, n_{k,t}^{\alpha_{k}}\,{\gamma_{k,z,t}}\,x_{k,z,t}^{-1}\prod_{j=1}^{M} x_{k,j,t}^{\gamma_{k,j}}=1
\end{dmath}
